\title{Imaging condition}
\author{Paul Sava}

\def\mt{\left( {\bf m},t \right)}
\def\mm{\left( {\bf m}   \right)}
\def\Us{U_s}
\def\Ur{U_r}
\def\R {R  }

\[\Us = \Us\mt \]
\[\Ur = \Ur\mt \]
\[\R  = \R \mm \]

\subsection{Imaging 1}
\[ \R = \int \Ur \Us dt \]

\subsection{Imaging 2}
\[ \R = \int \frac{\Ur \Us}{\Us^2 + \epsilon^2} dt \]

\subsection{Imaging 3}
\[ \R = \frac{\int \Ur \Us dt}{\int \Us^2 dt + \epsilon^2} \]

\subsection{Imaging 4}
\[ \R = \frac{\int \Ur \Us dt}
                {\sqrt{\int \Us^2 dt \int \Ur^2 dt}} \]

\subsection{Imaging 5}
\[ \R = \frac{                             \left( \int \Ur \Us   dt \right)^3}
             {\left( \int \Us^2 dt \right) \left( \int \Ur \Us   dt \right)^2 +
              \epsilon^2                   \left( \int     \Us^2 dt \right)^2}
\]

%****
%^^
